Kraken/AArch64/Sep.lean
@@ -8,25 +8,26 @@ open List
 
 @[kspec]
 theorem store_sep {α : Type} (s : MachineData) (addr : BitVec 64) (w : MemWidth)
-    (v : w.type) (ret : MachineData → Effects α)
+    (v : w.type) (k : MachineData → Effects α)
     (bs : List UInt8) (R : DataMem → Prop)
     (h_mem : s.dmem =⋆ Eq (bs.At addr) ⋆ R)
     (h_len : bs.length = w.bytes) :
     have mem' := Mem.storeInt s.dmem addr w.bytes v.toInt
-    MachineData.store s addr v ret =
+    (MachineData.store s addr v).bind k =
       require_write_access addr w (fun _ =>
-        ret { s with dmem := mem' }) := by
+        k { s with dmem := mem' }) := by
   have h_load : Mem.loadInt s.dmem addr w.bytes = some (Int.ofBytes bs) :=
     Mem.loadInt_sep bs addr w.bytes R s.dmem h_mem h_len (by cases w <;> decide)
-  simp only [MachineData.store, h_load]
+  simp only [MachineData.store, h_load, Effects.bind]
 
 @[kspec]
 theorem load_sep {α : Type} (s : MachineData) (addr : BitVec 64) (w : MemWidth)
-    (ret : w.type → MachineData → Effects α)
+    (k : w.type × MachineData → Effects α)
     (bs : List UInt8) (R : DataMem → Prop)
     (h_mem : s.dmem =⋆ Eq (bs.At addr) ⋆ R)
     (h_len : bs.length = w.bytes) :
-    MachineData.load s addr w ret =
-      require_read_access addr w (fun _ => ret (.ofInt w.bits (Int.ofBytes bs)) s) := by
+    (MachineData.load s addr w).bind k =
+      require_read_access addr w (fun _ => k (.ofInt w.bits (Int.ofBytes bs), s)) := by
   simp only [MachineData.load,
-    Mem.loadInt_sep bs addr w.bytes R s.dmem h_mem h_len (by cases w <;> decide)]
+    Mem.loadInt_sep bs addr w.bytes R s.dmem h_mem h_len (by cases w <;> decide),
+    Effects.bind]
